theories/typing.v
@@ -1,7 +1,7 @@
 Require Export imports.
 
 Reserved Notation "Γ ⊢ a ∈ A" (at level 70).
-
+Reserved Notation "Γ ⊢ a ≡ b ∈ A" (at level 70).
 Inductive Wt Γ : Tm -> Ty -> Prop :=
 | T_Var i A :
   lookup i Γ A ->
@@ -14,3 +14,28 @@ Inductive Wt Γ : Tm -> Ty -> Prop :=
   A::Γ ⊢ b ∈ B ->
   Γ ⊢ Abs b ∈ Fun A B
 where "Γ ⊢ a ∈ A" := (Wt Γ a A).
+
+Inductive Eq Γ : Tm -> Tm -> Ty -> Prop :=
+| J_Refl a A :
+  Γ ⊢ a ∈ A ->
+  Γ ⊢ a ≡ a ∈ A
+| J_Sym a b A :
+  Γ ⊢ a ≡ b ∈ A ->
+  Γ ⊢ b ≡ a ∈ A
+| J_Trans a b c A :
+  Γ ⊢ a ≡ b ∈ A ->
+  Γ ⊢ b ≡ c ∈ A ->
+  Γ ⊢ a ≡ c ∈ A
+| J_App b0 b1 a0 a1 A B :
+  Γ ⊢ b0 ≡ b1 ∈ Fun A B ->
+  Γ ⊢ a0 ≡ a1 ∈ A ->
+  Γ ⊢ App b0 a0 ≡ App b1 a1 ∈ B
+| J_β b a A B :
+  A :: Γ ⊢ b ∈ B ->
+  Γ ⊢ a ∈ A ->
+  Γ ⊢ App (Abs b) a ≡ b[a..] ∈ B
+| J_η a b A B :
+  A :: Γ ⊢ App a⟨shift⟩ (VarTm var_zero) ≡
+    App b⟨shift⟩ (VarTm var_zero) ∈ B ->
+  Γ ⊢ a ≡ b ∈ Fun A B
+where "Γ ⊢ a ≡ b ∈ A" := (Eq Γ a b A).
